theories/Compositional_Structures/Basic_Modules/Condorcet_Module_Ref.thy
@@ -3,7 +3,7 @@ theory Condorcet_Module_Ref
            "Component_Types/Elimination_Module_Ref"
 begin
 
-fun condorcet_score_ref :: "'a Evaluation_Function_Ref" where
+definition condorcet_score_ref :: "'a Evaluation_Function_Ref" where
   "condorcet_score_ref x A p = do {
     is_x_cond_winner <- (condorcet_winner_monadic A p x);
     RETURN (if (is_x_cond_winner) then 1 else 0)}"
@@ -15,32 +15,17 @@ definition condorcet_ref :: "'a Electoral_Module_Ref" where
    max_eliminator_ref scores A pl
 }"
 
-lemma condorcet_score_correct:
-  shows "(condorcet_score_ref, condorcet_score)
-    \<in> evalf_rel_prof"
-  unfolding evalf_rel_prof_def
-proof (clarify, refine_rcg, unfold condorcet_score_ref.simps condorcet_score.simps, refine_vcg,
-    rename_tac x A' pl A pr)
-  fix A' A :: "'a set"
-  fix x :: 'a
-  fix pl :: "'a Profile_List"
-  fix pr :: "'a Profile"
-  assume aprel: "((A', pl), A, pr) \<in> \<langle>Id\<rangle>alt_and_profile_rel" 
-  from aprel have finA: "finite A" unfolding alt_and_profile_rel_def
-    by (simp add: finite_set_rel_def in_br_conv)
-  from aprel have prel: "(pl, pr) \<in> profile_on_A_rel A" unfolding alt_and_profile_rel_def
-    by (simp add: finite_set_rel_def in_br_conv)
-  show "condorcet_winner_monadic A' pl x
-       \<le> SPEC (\<lambda>is_x_cond_winner.
-                   RETURN (if is_x_cond_winner then 1 else 0)
-                   \<le> SPEC (\<lambda>sc. sc = (if condorcet_winner A pr x then 1 else 0)))"
-    using condorcet_winner_monadic_correct
-      IdI apply (auto simp del: condorcet_winner.simps)
-     apply (metis RES_sng_eq_RETURN RETURN_rule SPEC_trans aprel)
-    by (metis (mono_tags, lifting) SPEC_cons_rule aprel singleton_conv2)
-qed
-
-
+lemma condorcet_score_ref_correct:
+  fixes A:: "'a set"
+  fixes pl:: "'a Profile_List" and pr:: "'a Profile"
+  assumes 
+    fina: "finite A"
+    and profrel: "(pl, pr) \<in> profile_rel"
+    and profpropl: "profile_l A pl"
+  shows "condorcet_score_ref x A pl \<le> SPEC (\<lambda> sc. sc = (condorcet_score x A pr))"
+  unfolding condorcet_score_ref_def condorcet_score.simps
+  apply (refine_vcg assms condorcet_winner_monadic_correct)
+  by auto
 
 
 context fixed_alts 
@@ -50,7 +35,7 @@ sepref_definition condorcet_elim_sepref is
   "uncurry condorcet_ref":: 
   "alts_set_impl_assn\<^sup>k *\<^sub>a profile_impl_assn\<^sup>k 
    \<rightarrow>\<^sub>a (result_impl_assn)"
-  unfolding condorcet_ref_def  max_eliminator_ref_def condorcet_score_ref.simps 
+  unfolding condorcet_ref_def  max_eliminator_ref_def condorcet_score_ref_def 
     less_eliminator_ref_def  elimination_module_ref_def[abs_def] eliminate_def[abs_def]
     pre_compute_scores_def[abs_def] scoremax_def[abs_def] 
     condorcet_winner_monadic_def[abs_def]  wins_monadic_def[abs_def] prefer_count_monadic_imp_def
@@ -71,12 +56,10 @@ sepref_definition condorcet_elim_sepref is
   done
 
 
-
-
 theorem condorcet_ref_correct:
   shows "(condorcet_ref,  (RETURN oo condorcet)) \<in> 
   elec_mod_fixed_alts_rel"
-proof (unfold condorcet_ref_def, refine_vcg, auto simp only: in_br_conv set_rel_id prod_rel_id finite_set_rel_def,
+proof (unfold condorcet_ref_def condorcet.simps, refine_vcg, auto simp only: in_br_conv set_rel_id prod_rel_id finite_set_rel_def,
     rule refine_IdI, unfold comp_apply SPEC_eq_is_RETURN(2)[symmetric] , rename_tac pl pr)
   fix pl :: "nat Profile_List"
   fix pr :: "nat Profile"
@@ -84,32 +67,29 @@ proof (unfold condorcet_ref_def, refine_vcg, auto simp only: in_br_conv set_rel_
   assume fina: "finite Alts"
   from profrel have prel: "(pl, pr) \<in> profile_rel" using
       profile_type_ref by blast
-  from fina have arel: "(Alts, Alts) \<in> \<langle>Id\<rangle>finite_set_rel" using finite_set_rel_def
-    set_rel_id in_br_conv
-    by (metis Id_O_R )    
-  from this profrel have combrel: "((Alts,pl), Alts, pr) \<in> \<langle>Id\<rangle>alt_and_profile_rel"
-    using alt_and_profile_rel_def
+  from profrel have profpl: "profile_l Alts pl" using profile_prop_list by blast
+  from fina prel profpl  have 
+  "\<forall>a\<in>Alts. condorcet_score_ref a Alts pl \<le> SPEC (\<lambda>score. score = condorcet_score a Alts pr)"
+    using condorcet_score_ref_correct
+    by metis
+  from this prel fina  have  precompcond: "pre_compute_scores condorcet_score_ref Alts pl
+  \<le> SPEC (\<lambda>map. map = pre_computed_map condorcet_score Alts pr)" using
+    compute_scores_correct
     by blast
-  note csc = compute_scores_correct_prof[THEN fun_relD, THEN fun_relD, THEN nres_relD,
-      THEN refine_IdD]
-
-  have scorec: "(pre_compute_scores condorcet_score_ref Alts pl)
-    \<le> SPEC (\<lambda>map. map = pre_computed_map condorcet_score Alts pr)"
-    using condorcet_score_correct combrel csc[where x3 = condorcet_score_ref
-        and x'3 = condorcet_score and x2 = "(Alts, pl)" and x'2 = "(Alts, pr)"]
-    by auto
-
-  note maxc = max_eliminator_Id[THEN fun_relD, THEN nres_relD, THEN refine_IdD]
-
-  show "  pre_compute_scores condorcet_score_ref Alts pl \<bind> (\<lambda>scores. max_eliminator_ref scores Alts pl)
-       \<le> SPEC (\<lambda>x. x = condorcet Alts pr)" unfolding condorcet.simps
-    using  prel arel  scorec  maxc[where x2 = Alts and x'2 = Alts and pl3 = pl and pr3 = pr
-        and efn3 = condorcet_score]
-      specify_left[where m = "pre_compute_scores condorcet_score_ref Alts pl"
-        and f = "(\<lambda>scores. max_eliminator_ref scores Alts pl)"
-        and M = "SPEC (\<lambda>x. x = max_eliminator condorcet_score Alts pr)"
-        and \<Phi> = "(\<lambda>map. map = pre_computed_map condorcet_score Alts pr)"]
+  note maxelim = max_eliminator_ref_correct[where efn = condorcet_score and A = Alts and pl = pl
+      and pr = pr]
+  from fina prel this have mid: "(\<And>x. x = pre_computed_map condorcet_score Alts pr \<Longrightarrow>
+          max_eliminator_ref x Alts pl \<le> SPEC (\<lambda>x. x = max_eliminator condorcet_score Alts pr))"
     by blast
+   show "pre_compute_scores condorcet_score_ref Alts pl \<bind> (\<lambda>scores. max_eliminator_ref scores Alts pl)
+       \<le> SPEC (\<lambda>x. x = max_eliminator condorcet_score Alts pr)"
+     unfolding comp_apply SPEC_eq_is_RETURN(2)[symmetric] 
+     apply refine_vcg
+     using precompcond  mid
+       SPEC_cons_rule[where m = "pre_compute_scores condorcet_score_ref Alts pl" and
+\<Psi> = "(\<lambda>scores. max_eliminator_ref scores Alts pl \<le> SPEC (\<lambda>x. x = max_eliminator condorcet_score Alts pr))"
+  and \<Phi> = "(\<lambda> map. map = (pre_computed_map condorcet_score Alts pr))"]
+     by blast 
 qed 
 
 term "(condorcet_ref,  (RETURN oo condorcet))"
