theories/Compositional_Structures/Loop_Composition_Ref.thy
@@ -1,0 +1,23 @@
+theory Loop_Composition_Ref
+  imports "Verified_Voting_Rule_Construction.Loop_Composition"
+      "Basic_Modules/Component_Types/Electoral_Module_Ref"
+
+begin
+
+function loop_comp_helper ::
+    "'a Electoral_Module \<Rightarrow> 'a Electoral_Module \<Rightarrow>
+        'a Termination_Condition \<Rightarrow> 'a Electoral_Module" where
+  "t (acc A p) \<or> \<not>((defer (acc \<triangleright> m) A p) \<subset> (defer acc A p)) \<or>
+    infinite (defer acc A p) \<Longrightarrow>
+      loop_comp_helper acc m t A p = acc A p" |
+  "\<not>(t (acc A p) \<or> \<not>((defer (acc \<triangleright> m) A p) \<subset> (defer acc A p)) \<or>
+    infinite (defer acc A p)) \<Longrightarrow>
+      loop_comp_helper acc m t A p = loop_comp_helper (acc \<triangleright> m) m t A p"
+
+definition loop_composition_ref :: "'a Electoral_Module \<Rightarrow> 'a Electoral_Module_Ref \<Rightarrow>
+        'a Termination_Condition \<Rightarrow> 'a Electoral_Module"
+  where   "loop_composition_ref \<equiv> do {
+    RETURN ({},{},{})
+}"
+
+end
